more proofs!

theories/Lambda/Red.v
@@ -27,6 +27,8 @@ Section substitute.
           {T2Ok : Typ2Ok T2}
           {RSOk : RSymOk RS}.
 
+  Context {ED_typ : EqDec _ (@eq typ)}.
+
   Fixpoint substitute' (v : var) (w : expr typ sym) (e : expr typ sym)
   : expr typ sym :=
     match e with
@@ -43,14 +45,35 @@ Section substitute.
     end.
 
   Theorem substitute'_typed
-  : forall ts tus e tvs w tvs' t t',
+  : forall ts tus t e w tvs' tvs t',
       typeof_expr ts tus (tvs ++ tvs') w = Some t ->
       typeof_expr ts tus (tvs ++ t :: tvs') e = Some t' ->
       typeof_expr ts tus (tvs ++ tvs') (substitute' (length tvs) w e) = Some t'.
   Proof.
     induction e; simpl; intros;
     forward; inv_all; subst; Cases.rewrite_all_goal; auto.
-  Admitted.
+    { consider (nat_compare (length tvs) v).
+      { intros. apply nat_compare_eq in H1.
+        subst. rewrite nth_error_app_R in H0.
+        replace (length tvs - length tvs) with 0 in H0 by omega.
+        simpl in *. inversion H0. subst; auto.
+        omega. }
+      { intros. apply nat_compare_lt in H1.
+        simpl.
+        rewrite nth_error_app_R in H0 by omega.
+        rewrite nth_error_app_R by omega.
+        change (t :: tvs') with ((t :: nil) ++ tvs') in H0.
+        rewrite nth_error_app_R in H0. 2: simpl; omega.
+        simpl in *. rewrite <- H0. f_equal. omega. }
+      { intros. apply nat_compare_gt in H1.
+        simpl. rewrite nth_error_app_L in * by omega. assumption. } }
+    { eapply (IHe (lift 0 1 w) tvs' (t0 :: tvs)) in H0; eauto.
+      simpl in *. rewrite H0. reflexivity.
+      simpl.
+      generalize (typeof_expr_lift ts tus w nil (t0 :: nil) (tvs ++ tvs')).
+      simpl.
+      intro. rewrite H1. assumption. }
+  Qed.
 
   Theorem substitute'_sound
   : forall ts tus e tvs w e',
@@ -82,13 +105,75 @@ Section substitute.
         simpl. inversion 1. subst. clear x1.
         destruct r. rewrite H0. intros.
         rewrite H. unfold Rcast_val, Rcast, Relim. simpl.
-        clear.
         rewrite hlist_nth_hlist_app; eauto.
-        admit. admit. }
+        generalize (cast1 tvs (x :: tvs') (length tvs)).
+        generalize (cast2 tvs (x :: tvs') (length tvs)).
+        clear - ED_typ.
+        rewrite x0.
+        replace (length tvs - length tvs) with 0 by omega.
+        simpl in *.
+        generalize dependent (o us (hlist_app gs gs')).
+        generalize dependent (hlist_nth gs (length tvs)).
+        gen_refl.
+        cutrewrite (nth_error tvs (length tvs) = None).
+        { intros. generalize (e0 e). unfold value. uip_all'. reflexivity. }
+        { rewrite nth_error_past_end; auto. } }
       { apply nat_compare_lt in H.
-        admit. }
+        autorewrite with exprD_rw; simpl.
+        eapply nth_error_get_hlist_nth_appR in H2; simpl in *; [ | omega ].
+        destruct H2.
+        consider (v - length tvs).
+        { intro. exfalso. omega. }
+        { intros. assert (n = (v - 1) - length tvs) by omega; subst.
+          forward.
+          assert (v - 1 >= length tvs) by omega.
+
+          eapply (@nth_error_get_hlist_nth_rwR _ (typD ts) tvs tvs') in H6.
+          rewrite H4 in *. forward_reason.
+          rewrite H6. subst. inv_all; subst. subst.
+          destruct r. rewrite type_cast_refl; eauto.
+          intros. f_equal. rewrite H8. apply H7. } }
       { apply nat_compare_gt in H.
-        admit. } }
+        autorewrite with exprD_rw; simpl.
+        assert (v < length tvs) by omega.
+        generalize H1.
+        eapply (@nth_error_get_hlist_nth_appL _ (typD ts) (t :: tvs')) in H1.
+        intro.
+        eapply (@nth_error_get_hlist_nth_appL _ (typD ts) tvs') in H4.
+        forward_reason. Cases.rewrite_all_goal.
+        destruct x0; simpl in *.
+        rewrite H7 in H5. inv_all; subst. destruct r.
+        repeat match goal with
+                 | H : _ |- _ => eapply nth_error_get_hlist_nth_Some in H
+               end; simpl in *; forward_reason.
+        unfold Rcast_val, Rcast in *; simpl in *.
+        consider (type_cast ts (projT1 x1) x).
+        { intros. red in r. subst. simpl.
+          rewrite H2; clear H2.
+          rewrite H4; clear H4.
+          clear - ED_typ H.
+          rewrite hlist_nth_hlist_app; eauto. symmetry.
+          rewrite hlist_nth_hlist_app; eauto.
+          gen_refl.
+          generalize dependent (hlist_nth gs v).
+          generalize (hlist_nth gs' (v - length tvs)).
+          generalize (hlist_nth (Hcons (o us (hlist_app gs gs')) gs')
+                                (v - length tvs)).
+          generalize (cast1 tvs (t :: tvs') v).
+          generalize (cast2 tvs (t :: tvs') v).
+          generalize (cast2 tvs tvs' v).
+          generalize (cast1 tvs tvs' v).
+          consider (nth_error tvs v).
+          { intros. generalize (e t0 e3).
+            generalize (e2 t0 e3). uip_all'.
+            clear - ED_typ. assert (t0 = projT1 x1) by congruence. subst.
+            uip_all'. reflexivity. }
+          { intros.
+            eapply nth_error_length_ge in H0. exfalso. omega. } }
+        { intros. eapply type_cast_total in H7; eauto.
+          apply H7. clear - x3 x5 H.
+          rewrite nth_error_app_L in * by omega.
+          rewrite x5 in x3. congruence. } } }
     { simpl. autorewrite with exprD_rw.
       unfold funcAs in *.
       generalize dependent (symD f).
@@ -98,13 +183,36 @@ Section substitute.
         simpl in *. unfold Rcast in H1. simpl in *. inv_all; subst; auto. }
       { congruence. } }
     { autorewrite with exprD_rw. simpl.
-      admit. }
+      erewrite substitute'_typed; eauto.
+      { specialize (IHe2 tvs w _ eq_refl tvs' t t0).
+        specialize (IHe1 tvs w _ eq_refl tvs' t (typ2 t0 t')).
+        revert IHe1 IHe2.
+        Cases.rewrite_all_goal. intros; forward.
+        unfold Open_App, OpenT, ResType.OpenT.
+        repeat first [ rewrite eq_Const_eq | rewrite eq_Arr_eq ].
+        rewrite IHe1. rewrite IHe2. reflexivity. }
+      { eapply exprD'_typeof_expr.
+        left. eauto. } }
     { autorewrite with exprD_rw. simpl.
       destruct (typ2_match_case ts t').
       { destruct H as [ ? [ ? [ ? ? ] ] ].
         rewrite H in *; clear H.
-        admit. }
-      { admit. } }
+        red in x1. subst. simpl in *.
+        destruct (eq_sym (typ2_cast ts x x0)).
+        forward. inv_all; subst.
+        specialize (IHe (t :: tvs) (lift 0 1 w) _ eq_refl tvs' t0 x0).
+        revert IHe. simpl.
+        generalize (exprD'_lift ts tus w nil (t :: nil) (tvs ++ tvs') t0).
+        simpl. Cases.rewrite_all_goal.
+        intros. forward.
+        eapply functional_extensionality. intros.
+        unfold Rcast_val, Rcast; simpl.
+        inv_all; subst.
+        specialize (IHe us (Hcons x1 gs)). simpl in *.
+        specialize (H3 us Hnil). simpl in *.
+        erewrite H3. instantiate (1 := Hcons x1 Hnil).
+        eapply IHe. }
+      { rewrite H in *. congruence. } }
     { autorewrite with exprD_rw. simpl.
       rewrite H2. rewrite H3. auto. }
   Qed.
@@ -187,6 +295,7 @@ Section beta.
       { split; auto.
         clear H5. unfold Open_App.
         repeat first [ rewrite eq_Const_eq | rewrite eq_Arr_eq ].
+        generalize (@substitute'_sound).
         admit. } }
     { intros. forward_reason.
       forward. simpl.
@@ -210,6 +319,8 @@ Section beta_all.
   Context {RTOk : RTypeOk _}
           {T2Ok : Typ2Ok T2}
           {RSOk : RSymOk RS}.
+
+  Context {ED_typ : EqDec _ (@eq typ)}.
 
   (** NOTE: I should extend [delta] with [vars]
    ** - that means that its specification is exactly the same as [beta_all]
@@ -258,6 +369,50 @@ Section beta_all.
                        @EnvForall A R es ts vs ->
                        @EnvForall A R (e :: es) (t :: ts) (Hcons v vs).
 
+  Lemma Forall2_sem2
+  : forall T U (P : T -> U -> Prop) xs ys,
+      Forall2 P xs ys ->
+      forall v y,
+        nth_error ys v = Some y ->
+        exists x, nth_error xs v = Some x /\
+                  P x y.
+  Proof.
+    clear. induction 1; simpl; intros.
+    { destruct v; inversion H. }
+    { destruct v.
+      { simpl in *. eexists; split; eauto.
+        inversion H1. subst. auto. }
+      { simpl in *. eauto. } }
+  Qed.
+
+  Section Forall2i.
+    Variables T U : Type.
+
+    Section def.
+      Variable P : nat -> T -> U -> Prop.
+
+      Inductive Forall2i : nat -> list T -> list U -> Prop :=
+      | F2i_nil : forall n, Forall2i n nil nil
+      | F2i_cons : forall x xs y ys n, P n x y ->
+                                       Forall2i (S n) xs ys ->
+                                       Forall2i n (x :: xs) (y :: ys).
+    End def.
+
+    Variable P Q : nat -> T -> U -> Prop.
+    Lemma Forall2i_shift
+    : forall m n xs ys,
+        (forall n x y, P n x y -> Q (m + n) x y) ->
+        Forall2i P n xs ys ->
+        Forall2i Q (m + n) xs ys.
+    Proof.
+      clear. induction 2.
+      { constructor. }
+      { constructor; eauto.
+        replace (m + S n) with (S (m + n)) in IHForall2i by omega.
+        assumption. }
+    Qed.
+  End Forall2i.
+
 (*
   Lemma beta_all_respectful
   : forall args args' vars vars' e e',
@@ -266,13 +421,59 @@ Section beta_all.
       beta_all args' vars' e'
 *)
 
+  Lemma eq_sym_eq_sym : forall T (a b : T) (pf : a = b),
+                          eq_sym (eq_sym pf) = pf.
+  Proof.
+    clear. destruct pf. reflexivity.
+  Qed.
+
+  Lemma eq_eq_sym : forall T F (a b : T) (pf : a = b) (x : F b),
+                      match pf in _ = t return F t with
+                        | eq_refl =>
+                          match eq_sym pf in _ = t return F t with
+                            | eq_refl => x
+                          end
+                      end = x.
+  Proof.
+    clear. destruct pf. reflexivity.
+  Qed.
+
+  Lemma exprD'_App_Abs
+  : forall ts tus tvs t t0 e ex val,
+      exprD' ts tus tvs t0 (App (Abs t e) ex) = Some val ->
+      exprD' ts tus tvs t0 (substitute' 0 ex e) = Some val.
+  Proof.
+    intros.
+    autorewrite with exprD_rw in *; simpl in *.
+    forward.
+    autorewrite with exprD_rw in *; simpl in *.
+    inv_all; subst.
+    rewrite typ2_match_zeta in H0; eauto.
+    rewrite eq_option_eq in H0.
+    forward. inv_all; subst.
+    destruct r.
+    generalize (@substitute'_sound _ _ _ _ _ _ _ _ ts0 tus e nil ex _ eq_refl tvs t1 t0).
+    simpl. Cases.rewrite_all_goal.
+    intros. forward.
+    f_equal. unfold Open_App.
+    unfold OpenT, ResType.OpenT.
+    repeat first [ rewrite eq_Const_eq | rewrite eq_Arr_eq ].
+    clear - H4.
+    apply functional_extensionality; intro.
+    apply functional_extensionality; intro.
+    repeat first [ rewrite eq_Const_eq | rewrite eq_Arr_eq ].
+    specialize (H4 x Hnil x0).
+    simpl in *.
+    rewrite eq_sym_eq_sym. rewrite eq_eq_sym. auto.
+  Qed.
+
   Theorem beta_all_sound
   : forall tus e tvs t val args vars,
-      Forall2 (fun t e => match e with
-                            | None => True
-                            | Some e =>
-                              exists val, exprD' ts tus tvs t e = Some val
-                          end) tvs vars ->
+      Forall2i (fun n t e => match e with
+                               | None => True
+                               | Some e =>
+                                 exists val, exprD' ts tus (skipn n tvs) t e = Some val
+                             end) 0 tvs vars ->
       exprD' ts tus tvs t (apps e args) = Some val ->
       exists val',
         exprD' ts tus tvs t (beta_all args vars e) = Some val' /\
@@ -287,7 +488,12 @@ Section beta_all.
           val us vs = val' us vs.
   Proof.
     induction e; simpl; intros.
-    { admit. }
+    { (*consider (nth_error vars v).
+       { destruct o; intros.
+        {           eapply Forall2_sem2 in H1; eauto. simpl in *.
+
+
+        *) admit. }
     { eapply deltaOk in H0.
       destruct H0 as [ ? [ ? ? ] ].
       eexists; split; eauto. }
@@ -297,13 +503,48 @@ Section beta_all.
       forward.
       autorewrite with exprD_rw in *; simpl in *; forward.
       change e2 with (apps e2 nil) in H5.
-      eapply IHe2 with (vars := vars) in H5; eauto.
+      eapply IHe2 with (vars := vars) in H5; eauto; clear IHe2.
       forward_reason.
-      change (apps (App e1 e2) args)
-        with (apps e1 (e2 :: args)) in H2.
-      eapply IHe1 in H2; eauto.
-      revert deltaOk. admit. }
-    { admit. }
+      assert (exists val',
+                exprD' ts tus tvs t (apps (App e1 (beta_all nil vars e2)) args) = Some val' /\
+             forall us vs,
+               EnvForall
+                 (fun (e : option (expr typ sym)) (t3 : typ) (v : typD ts t3) =>
+                    match e with
+                      | Some e0 =>
+                        exists val0 : OpenT ts tus tvs (typD ts t3),
+                                      exprD' ts tus tvs t3 e0 = Some val0 /\ val0 us vs = v
+                      | None => True
+                    end) vars vs ->
+               val us vs = val' us vs).
+      { admit. }
+      destruct H9 as [ ? [ ? ? ] ].
+      change (apps (App e1 (beta_all nil vars e2)) args)
+        with (apps e1 (beta_all nil vars e2 :: args)) in H9.
+      eapply IHe1 in H9; eauto.
+      forward_reason. eexists; split; eauto.
+      intros. rewrite <- H11; eauto. }
+    { destruct args.
+      { simpl in *.
+        autorewrite with exprD_rw in *; simpl in *.
+        Require Import MirrorCore.Lambda.ExprTac.
+        arrow_case ts t0.
+        { clear H1. red in x1. subst. simpl in *.
+          rewrite eq_option_eq in *.
+          forward. inv_all; subst.
+          change e with (apps e nil) in H2.
+          eapply IHe with (vars := None :: vars) in H2; eauto.
+          { admit. }
+          { constructor; auto.
+            revert H.
+            eapply (@Forall2i_shift _ _ _ _ 1 0). intros.
+            simpl; auto. } }
+        { congruence. } }
+      { simpl in *.
+        rewrite exprD'_apps in H0; eauto.
+        unfold apps_sem' in H0; eauto. forward.
+        eapply exprD'_App_Abs in H1; eauto.
+        admit. } }
     { eapply deltaOk in H0.
       forward_reason. eauto. }
   Qed.
